theories/SMTLibFacts.v
@@ -1,117 +1,57 @@
 Require List.
 Import List.ListNotations.
+Require Import Morphisms.
 
 Require Import SMTLib.
 
-Fixpoint term_domain (t : SMTLib.term) : list const_sym :=
-  match t with
-  | SMTLib.Term_Const sym => [sym]
-  | SMTLib.Term_Int _ => []
-  | SMTLib.Term_Geq l r => (term_domain l) ++ (term_domain r)
-  | SMTLib.Term_Eq l r => (term_domain l) ++ (term_domain r)
-  | SMTLib.Term_And l r => (term_domain l) ++ (term_domain r)
-  | SMTLib.Term_Or l r => (term_domain l) ++ (term_domain r)
-  | SMTLib.Term_Not e => term_domain e
-  | SMTLib.Term_ITE c t f => (term_domain c) ++ (term_domain t) ++ (term_domain f)
-  | SMTLib.Term_True => []
-  | SMTLib.Term_False => []
-  | SMTLib.Term_BVLit _ _ => []
-  | SMTLib.Term_BVConcat l r => (term_domain l) ++ (term_domain r)
-  | SMTLib.Term_BVExtract _ _ e => term_domain e
-  | SMTLib.Term_BVUnaryOp _ e => term_domain e
-  | SMTLib.Term_BVBinOp _ l r => (term_domain l) ++ (term_domain r)
-  | SMTLib.Term_BVUlt l r => (term_domain l) ++ (term_domain r)
-  end
-.
-
-Definition domain (q : query) : list const_sym := List.concat (List.map term_domain q).
-
-Definition list_disjoint {A} (l1 l2 : list A) :=
-  forall x, (List.In x l1 -> ~ List.In x l2) /\ (List.In x l2 -> ~ List.In x l1).
-
-Lemma list_disjoint_cons {A} (a : A) l1 l2 :
-  list_disjoint (a :: l1) l2 -> list_disjoint l1 l2.
-Proof.
-  unfold list_disjoint in *.
-  intros H; split.
-  - destruct H with x; intuition eauto with datatypes.
-  - destruct H with x; intuition eauto with datatypes.
-Qed.
-
-Lemma list_disjoint_concat {A} (l1 l2 l3 : list A) :
-  list_disjoint (l1 ++ l2) l3 -> list_disjoint l2 l3.
-Proof.
-  revert l2 l3.
-  induction l1.
-  - trivial.
-  - intros.
-    rewrite <- List.app_comm_cons in H.
-    apply list_disjoint_cons in H.
-    eauto.
-Qed.
-
-Definition disjoint (q1 q2 : query) := list_disjoint (domain q1) (domain q2).
-
-Lemma disjoint_cons (t : term) q1 q2 :
-  disjoint (t :: q1)%list q2 -> disjoint q1 q2.
-Proof.
-  unfold disjoint in *.
-  intros H.
-  unfold domain in H; simpl in H.
-  eapply list_disjoint_concat.
-  eassumption.
-Qed.
-
 Infix "⊧" := satisfied_by (at level 20).
-
-Lemma concat_same_model : forall q1 q2 ρ,
-    ρ ⊧ q1 ->
-    ρ ⊧ q2 ->
-    ρ ⊧ (q1 ++ q2)%list.
-Proof.
-  induction q1.
-  - intros.
-    simpl in *.
-    assumption.
-  - intros * Hq1 Hq2.
-    inversion Hq1; subst; clear Hq1.
-    rewrite <- List.app_comm_cons.
-    constructor; eauto.
-    apply IHq1; eauto.
-Qed.
 
 Definition smt_reflect (q: query) (P : valuation -> Prop): Prop :=
   forall ρ, ρ ⊧ q <-> P ρ.
+
+Lemma combine_wf q1 q2 :
+  List.Forall
+    (fun n : nat => exists s : sort, List.In (n, s) (declarations q1 ++ declarations q2))
+    (lst_domain (assertions q1 ++ assertions q2)).
+Proof.
+  destruct q1, q2.
+  unfold lst_domain in *.
+  rewrite ! List.Forall_forall in *.
+  simpl in *.
+  rewrite List.Forall_forall in *.
+  intros n H.
+  rewrite
+    <- List.flat_map_concat_map,
+    List.flat_map_app,
+    List.in_app_iff
+    in *.
+  setoid_rewrite List.in_app_iff.
+  destruct H.
+  - edestruct wf as [n' Hwf]. eapply H.
+    eauto.
+  - edestruct wf0 as [n' Hwf]. eapply H.
+    eauto.
+Qed.
+
+Definition combine (q1 q2: query) : query :=
+  {|
+    declarations := declarations q1 ++ declarations q2;
+    assertions := assertions q1 ++ assertions q2;
+    wf := combine_wf q1 q2
+  |}.
 
 Lemma concat_conj :
   forall q1 q2 P1 P2,
     smt_reflect q1 P1 ->
     smt_reflect q2 P2 ->
-    smt_reflect (q1 ++ q2)%list (fun ρ => P1 ρ /\ P2 ρ).
+    smt_reflect (combine q1 q2) (fun ρ => P1 ρ /\ P2 ρ).
 Proof.
-  induction q1; intros * * HPq1 HPq2.
-  - simpl. split. intros H.
-    + split.
-      * apply HPq1. constructor.
-      * apply HPq2. assumption.
-    + intros [HP1 HP2].
-      apply HPq2.
-      assumption.
-  - split.
-    + intros Hρ.
-      unfold "⊧" in Hρ.
-      rewrite List.Forall_app in Hρ; destruct Hρ.
-      fold (ρ ⊧ (a :: q1)%list) in *; fold (ρ ⊧ q2) in *.
-      split.
-      * apply HPq1. assumption.
-      * apply HPq2. assumption.
-    + intros [HP1 HP2].
-      unfold "⊧".
-      rewrite List.Forall_app.
-      fold (ρ ⊧ (a :: q1)%list) in *; fold (ρ ⊧ q2) in *.
-      split.
-      * apply HPq1. assumption.
-      * apply HPq2. assumption.
+  destruct q1, q2.
+  unfold smt_reflect, satisfied_by, combine.
+  simpl.
+  intros.
+  setoid_rewrite List.Forall_app.
+  firstorder.
 Qed.
 
 Local Open Scope list.
@@ -119,56 +59,11 @@ Local Open Scope list.
 Lemma unsat_smt_reflect_false q :
   UNSAT q <-> smt_reflect q (fun _ => False).
 Proof.
-  unfold UNSAT.
-  split.
-  - intros Hunsat.
-    split; intuition eauto.
-  - intros Hq * contra.
-    apply Hq in contra.
-    contradiction.
+  unfold UNSAT, smt_reflect, satisfied_by, combine.
+  simpl.
+  intros.
+  firstorder.
 Qed.
-
-Definition Qa := [ Term_Const 0 ].
-Definition a_is_true := (fun ρ => ρ 0 = Some (Value_Bool true)).
-Definition a_is_false := (fun ρ => ρ 0 = Some (Value_Bool false)).
-
-Lemma Qa_prop : smt_reflect Qa a_is_true.
-Proof.
-  unfold Qa, a_is_true.
-  split; intros.
-  - inversion H; subst; clear H.
-    inversion H2; subst; clear H2.
-    reflexivity.
-  - repeat constructor.
-    unfold term_satisfied_by; simpl.
-    rewrite H; clear H.
-    reflexivity.
-Qed.
-
-Definition Qnota := [ Term_Not (Term_Const 0) ].
-Lemma Qnota_prop : smt_reflect Qnota a_is_false.
-Proof.
-  unfold Qnota, a_is_false.
-  split; intros.
-  - inversion H; subst; clear H.
-    inversion H2; subst; clear H2.
-    destruct (ρ 0); try discriminate.
-    destruct v; try discriminate.
-    inversion H0.
-    symmetry in H1. apply Bool.negb_sym in H1. simpl in H1.
-    subst. reflexivity.
-  - repeat constructor.
-    unfold term_satisfied_by; simpl.
-    rewrite H; clear H.
-    reflexivity.
-Qed.
-
-Lemma Qa_Qnota_concat : smt_reflect (Qa ++ Qnota) (fun ρ => a_is_true ρ /\ a_is_false ρ).
-Proof. auto using concat_conj, Qa_prop, Qnota_prop. Qed.
-
-(* Global Instance x : Morphisms.Proper (Morphisms.pointwise_relation valuation iff => Basics.flip Basics.impl) (smt_reflect (Qa ++ Qnota)). *)
-
-Require Import Relation_Definitions Setoid.
 
 Lemma smt_reflect_rewrite : forall P2 P1 q,
     (forall ρ, P1 ρ <-> P2 ρ) ->
@@ -181,17 +76,6 @@ Proof.
     apply Hsmt_reflect.
   - rewrite HP.
     apply Hsmt_reflect.
-Qed.
-
-Lemma Qa_Qnota_unsat : UNSAT (Qa ++ Qnota).
-  apply unsat_smt_reflect_false.
-  rewrite (smt_reflect_rewrite (fun ρ => a_is_true ρ /\ a_is_false ρ)).
-  - apply Qa_Qnota_concat.
-  - split; try contradiction.
-    intros [Htrue Hfalse].
-    unfold a_is_true, a_is_false in *.
-    rewrite Htrue in Hfalse.
-    discriminate.
 Qed.
 
 Definition equisatisfiable q1 q2 := SAT q1 <-> SAT q2.
@@ -232,7 +116,7 @@ Qed.
 Lemma incompatible_reflect q1 q2 P1 P2 :
   smt_reflect q1 P1 ->
   smt_reflect q2 P2 ->
-  UNSAT (q1 ++ q2) ->
+  UNSAT (combine q1 q2) ->
   (forall ρ, ~ (P1 ρ /\ P2 ρ)).
 Proof.
   intros Hq1P1 Hq2P2 Hunsat.
